compiler/backend/proofs/source_evalProofScript.sml
@@ -643,6 +643,8 @@ Proof
     \\ Cases_on ‘test_ty’ \\ gvs [check_type_def]
     \\ res_tac
     \\ rename [‘WordT wt’] \\ Cases_on ‘wt’ \\ gvs [check_type_def])
+  >~ [‘do_airth’] >- cheat
+  >~ [‘do_conversion’] >- cheat
   >~ [`thunk_op`]
   >- (
     gvs [AllCaseEqs(), PULL_EXISTS, thunk_op_def]
